ROOT
@@ -4,8 +4,7 @@ session Graph in Graph = "HOL-Library" +
   description
     "GraalVM Intermediate Representation encoding"
   options [document = pdf, document_output = "output",
-           show_question_marks = false,
-           quick_and_dirty] (* Temporary sorry in Class for termination proof *)
+           show_question_marks = false]
   theories
     JavaWords
     JavaLong
@@ -26,8 +25,7 @@ session Semantics in Semantics = Graph +
   description
     "Semantics of the GraalVM IR"
   options [document = pdf, document_output = "output",
-           show_question_marks = false,
-           quick_and_dirty] (* IRStepObj imports Class, which is temporarily sorry'd *)
+           show_question_marks = false]
   sessions
     "HOL-Eisbach"
   theories
